src/go_lang/notation.v
@@ -110,6 +110,10 @@ Notation "e1 = e2" := (BinOp EqOp e1%E e2%E) : expr_scope.
 Notation "e1 ≠ e2" := (UnOp NegOp (BinOp EqOp e1%E e2%E)) : expr_scope.
 
 Notation "~ e" := (UnOp NegOp e%E) (at level 75, right associativity) : expr_scope.
+Definition Store {ext:ext_op} : val :=
+  LamV "l" (LamV "v" (Seq
+                      (PrepareWrite (Var "l"))
+                      (FinishStore (Var "l") (Var "v")))).
 (* The unicode ← is already part of the notation "_ ← _; _" for bind. *)
 Notation "e1 <- e2" := (Store e1%E e2%E) (at level 80) : expr_scope.
 
